

UWaterloo 2026 Winter PMATH352 - Complex Analysis

Instructor: Professor **Jason P. Bell**
Student: **Shao-Kai Jonathan Huang**

January 14, 2026

Contents

1 **Complex Differentiation**

2

1 Complex Differentiation

Date: 12/1/2026

Theorem 1.1 (Cauchy-Riemann). *Let f be a differentiable function from an open set $U \subseteq \mathbb{C}$ to \mathbb{C} . Write $f(z) = u(x, y) + iv(x, y)$, where $z = x + iy$, $u, v : U \rightarrow \mathbb{R}$. Then the partial derivatives of u and v satisfy the Cauchy-Riemann equations given by*

$$\frac{\partial u}{\partial x} = \frac{\partial v}{\partial y}, \quad \frac{\partial u}{\partial y} = -\frac{\partial v}{\partial x}. \quad (1)$$

This is a necessary condition for complex differentiability. To see why it is not sufficient, we can consider the following example.

Example 1.1 (Non-differentiability). Let $f(z)$ be defined by $z^5/|z|^4$ when $z \neq 0$

Date: 14/1/2026

Theorem 1.2. If $f(z) = \sum a_n z^n \in \mathbb{C}[[z]]$ has radius of convergence $R > 0$ and if $g(z) = \sum n a_n z^{n-1}$. Then $g(z)$ converges in $B(0, R)$ and $f'(z) = g(z)$ for all $z \in B(0, R)$.

Proof. We know from previous result that $g(z)$ has radius of convergence R . Now fix $z_0 \in B(0, R)$. There exists $\delta > 0$ such that $B(z_0, \delta) \subseteq B(0, R)$, so for all h such that $|h| < \delta$, $z_0 + h \in B(0, R)$. Let $h \in \mathbb{C}$, $0 < |h| < \delta$, consider

$$\begin{aligned}
 \left| \frac{f(z_0 + h) - f(z_0)}{h} - g(z_0) \right| &= \left| \frac{\sum_{n=0}^{\infty} a_n (z_0 + h)^n - \sum_{n=0}^{\infty} a_n z_0^n}{h} - \sum_{n=1}^{\infty} n a_n z_0^{n-1} \right| \\
 &= \left| \sum_{n=1}^{\infty} a_n \frac{(z_0 + h)^n - z_0^n}{h} - \sum_{n=1}^{\infty} n a_n z_0^{n-1} \right| \\
 &= \left| \sum_{n=1}^{\infty} a_n \left(\frac{(z_0 + h)^n - z_0^n}{h} - n z_0^{n-1} \right) \right| \\
 &= \left| \sum_{n=0}^{\infty} a_n \left[\sum_{j=2}^n \binom{n}{j} z_0^{n-j} h^{j-1} \right] \right| \\
 &\leq \sum_{n=0}^{\infty} |a_n| \sum_{j=2}^n \binom{n}{j} |z_0|^{n-j} |h|^{j-1} \\
 &\leq |h| \sum_{n=0}^{\infty} |a_n| \sum_{l=0}^{n-2} \binom{n}{2} \binom{n-2}{l} |z_0|^{n-2-l} |h|^l, \quad l = j - 2 \\
 &= |h| \sum_{n=2}^{\infty} |a_n| \binom{n}{2} (|z_0| + |h|)^{n-2} \\
 &\leq \frac{|h|}{2} \sum_{n=2}^{\infty} |a_n| n(n-1) \rho^{n-2} = C|h| \rightarrow 0, \quad \text{as } h \rightarrow 0.
 \end{aligned}$$

In the above derivation, we used the fact that the series $\sum_{n=0}^{\infty}$ is absolutely convergent, $|z_0| + |h| < |z_0| + \delta \leq \rho < R$. Therefore, the limit

$$\lim_{h \rightarrow 0} \left| \frac{f(z_0 + h) - f(z_0)}{h} \right|$$

exists and is equal to $g(z_0)$. Hence, for all $z \in B(0, R)$, we have

$$f'(z) = \sum_{n=1}^{\infty} n a_n z^{n-1}.$$

□

Corollary 1.3. If $f(z) = \sum_{n=0}^{\infty} a_n z^n$ is convergent in $B(0, R)$, then $f^{(j)}(z)$ exists and

$$\frac{f^{(j)}}{j!} = \sum_{n=j}^{\infty} \binom{n}{j} a_n z^{n-j}, \quad \text{for all } z \in B(0, R).$$

Definition 1.1. We define

$$\exp z = \sum_{n=0}^{\infty} \frac{z^n}{n!}, \quad \text{for all } z \in \mathbb{C}. \quad (2)$$

This power series has $R = \infty$.

Theorem 1.4. *The power series $\exp z$ has the following properties:*

- (i) $\exp x = e^x > 0$ for all $x \in \mathbb{R}$.
- (ii) $\exp \bar{z} = \overline{\exp z}$ for all $z \in \mathbb{C}$.
- (iii) $\exp(z + w) = \exp z \cdot \exp w$ for all $z, w \in \mathbb{C}$.
- (iv) $\frac{d}{dz} \exp z = \exp z$ for all $z \in \mathbb{C}$.
- (v) $|\exp z| = e^{\operatorname{Re}(z)}$ for all $z \in \mathbb{C}$.

Proof.

- (i) For $x \in \mathbb{R}$, we have $\exp x = \sum_{n=0}^{\infty} \frac{x^n}{n!} = e^x > 0$, by definition.
- (ii) If $S_N = \sum_{n=0}^N a_n \rightarrow S$, then $\overline{S_N} = \overline{\sum_{n=0}^N a_n} = \sum_{n=0}^N \overline{a_n} \rightarrow \overline{S}$. Therefore, $\exp \bar{z} = \overline{\exp z}$.
- (iii) Let $c \in \mathbb{C}$ and $f(z) = \exp(c - z) \exp z$. Assuming (iV) to be true, we have

$$\frac{d}{dz} f(z) = \exp(c - z) \exp z - \exp(c - z) \exp z = 0.$$

Therefore, $f(z)$ is constant. Evaluating at $z = 0$, we have $f(z) = f(0) = \exp c$. Let $c = z + w$, we get the desired result.

- (iv) By the corollary above, we have

$$\frac{d}{dz} \exp z = \sum_{n=1}^{\infty} \frac{n}{n!} z^{n-1} = \sum_{n=0}^{\infty} \frac{z^n}{n!} = \exp z.$$

- (v) we have

$$|\exp(z)|^2 = \exp z \overline{\exp z} = \exp z \exp \bar{z} = \exp(z + \bar{z}) = \exp(2 \operatorname{Re}(z)) = e^{2 \operatorname{Re}(z)}.$$

Therefore, $|\exp z| = e^{\operatorname{Re}(z)}$.

□

Definition 1.2 (Trigonometric functions). *We also define*

$$\sin z = \sum_{n=0}^{\infty} (-1)^n \frac{z^{2n+1}}{(2n+1)!}, \quad \cos z = \sum_{n=0}^{\infty} (-1)^n \frac{z^{2n}}{(2n)!}, \quad \text{for all } z \in \mathbb{C}. \quad (3)$$

These power series have $R = \infty$.

Corollary 1.5. *For all $z \in \mathbb{C}$, we have*

$$\frac{d}{dz} \sin z = \cos z, \quad \frac{d}{dz} \cos z = -\sin z. \quad (4)$$

Corollary 1.6 (Euler's identity). *For all $z \in \mathbb{C}$, we have*

$$\exp(iz) = \cos z + i \sin z. \quad (5)$$

Proof. Notice that $\exp(iz) = e^{iz} = 1 + iz + \frac{(iz)^2}{2!} + \frac{(iz)^3}{3!} + \cdots$ absolutely converges, so we may rearrange the terms as we wish. □